Semantic/ModalCapybara/Syntax.lean
@@ -1,7 +1,7 @@
 import Semantic.ModalCapybara.Syntax.Ty
 import Semantic.ModalCapybara.Syntax.Exp
 import Semantic.ModalCapybara.Syntax.Context
-import Semantic.ModalCapybara.Syntax.Constraint
+import Semantic.ModalCapybara.Syntax.SepCtx
 
 /-!
 Syntax definitions for CC.
