Semantic/ModalCapybara/Syntax/SepCtx.lean
@@ -1,0 +1,36 @@
+import Semantic.ModalCapybara.Syntax.CaptureSet
+
+namespace ModalCapybara
+
+/-- A separation constraint. -/
+inductive SepCtx : Sig -> Type where
+| empty : SepCtx s
+| cons :
+  SepCtx s ->
+  CaptureSet s ->
+  Mutability ->
+  SepCtx s
+
+/-- Applies a renaming to all bound variables in a separation context. -/
+def SepCtx.rename : SepCtx s1 -> Rename s1 s2 -> SepCtx s2
+| .empty, _ => .empty
+| .cons K C m, ρ => .cons (K.rename ρ) (C.rename ρ) m
+
+/-- Renaming by the identity renaming leaves a separation context unchanged. -/
+theorem SepCtx.rename_id {K : SepCtx s} :
+    K.rename Rename.id = K := by
+  induction K with
+  | empty => rfl
+  | cons K C m ih =>
+    simp [SepCtx.rename, ih, CaptureSet.rename_id]
+
+/-- Renaming distributes over composition of renamings. -/
+theorem SepCtx.rename_comp
+    {K : SepCtx s1} {f : Rename s1 s2} {g : Rename s2 s3} :
+    (K.rename f).rename g = K.rename (f.comp g) := by
+  induction K generalizing s2 s3 with
+  | empty => rfl
+  | cons K C m ih =>
+    simp [SepCtx.rename, ih, CaptureSet.rename_comp]
+
+end ModalCapybara
